

# Calculating Square Roots in $\mathbb{F}_{p^2}$

I present an exposition of the calculation of square roots in  $\mathbb{F}_{p^2}$ , where  $p$  is a prime with  $p \equiv -1 \pmod{4}$ , and  $\mathbb{F}_{p^2}$  is defined as  $\frac{\mathbb{F}_p[i]}{i^2+1}$ , so that elements of  $\mathbb{F}_{p^2}$  are of the form  $x + iy$ , with  $i^2 = -1$  and  $x, y \in \mathbb{F}_p$ .

**Definition 1.** For  $a \in \mathbb{F}_p$ , define the function  $L : \mathbb{F}_p \rightarrow \mathbb{F}_p$  as follows:

$$L(a) = \begin{cases} 1 & a \text{ is a non-zero square in } \mathbb{F}_p, \\ -1 & a \text{ is not a square in } \mathbb{F}_p, \\ 0 & a \equiv 0 \pmod{p}. \end{cases}$$

That is,  $L(a) = \left(\frac{a}{p}\right)$ , the Legendre symbol on  $p$ .

Recall the following elementary fact (which we can treat as an alternative definition of  $L$ ):

**Fact.** For all  $a \in \mathbb{F}_p$ ,  $L(a) \equiv a^{\frac{p-1}{2}} \pmod{p}$ .

**Remark.** Note that  $L(-1) \equiv -1 \pmod{p}$  by definition of  $p$ , and thus  $\mathbb{F}_{p^2}$  really is a quadratic extension of  $\mathbb{F}_p$ , as  $-1$  has no square root in  $\mathbb{F}_p$ .

We also define the following function.

**Definition 2.** For  $a \in \mathbb{F}_p$ , define the function  $K : \mathbb{F}_p \rightarrow \mathbb{F}_p$  by  $L(a) \equiv a^{\frac{p+1}{4}} \pmod{p}$

**Lemma 3.**  $K$  has the following properties:

- $K(a) \equiv 0 \pmod{p}$  if and only if  $a \equiv 0 \pmod{p}$ .
- $K(a)^2 \equiv aL(a) \pmod{p}$ .
- $K(a^2) \equiv aL(a) \pmod{p}$ .

*Proof.* The first property is trivial. For the second and third properties, simply note that  $aL(a) \equiv aa^{\frac{p-1}{2}} \equiv a^{\frac{p+1}{2}} \equiv (a^2)^{\frac{p+1}{4}} \equiv (a^{\frac{p+1}{4}})^2 \pmod{p}$ .  $\square$

**Remark.**  $K$ , of course, is a square root function for quadratic residues on  $\mathbb{F}_p$ , but we can define it over all of  $\mathbb{F}_p$ .

We now prove constructively a necessary and sufficient condition for  $s \in \mathbb{F}_{p^2}$  having a square root, and from that derive an algorithm for the calculation of square roots in  $\mathbb{F}_{p^2}$ .

**Theorem 4.** *Let  $s$  be a member of  $\mathbb{F}_{p^2}$ , with  $s = x + iy$ , with  $x, y \in \mathbb{F}_p$ . Then there exists an  $r \in \mathbb{F}_{p^2}$  such that  $r^2 = s$  if and only if  $L(x^2 + y^2) \neq -1$ .*

*Proof.* Suppose there exists such an  $r$ , and say  $r = \alpha + i\beta$ , with  $\alpha, \beta \in \mathbb{F}_p$ . Then  $r^2 = (\alpha^2 - \beta^2) + i(2\alpha\beta)$ , and so we must have  $x = \alpha^2 - \beta^2$  and  $y = 2\alpha\beta$ .

Define  $\bar{r} = \alpha - i\beta$ . Then

$$\bar{r}^2 = (\alpha^2 - \beta^2) - i(2\alpha\beta) = x - iy.$$

Note that  $r\bar{r} = \alpha^2 + \beta^2$ . It follows that

$$(\alpha^2 + \beta^2)^2 = (r\bar{r})^2 = r^2\bar{r}^2 = (x + iy)(x - iy) = x^2 + y^2.$$

This shows that  $x^2 + y^2$  is a square, and thus  $L(x^2 + y^2) \neq -1$ .

Conversely, suppose  $L(x^2 + y^2) \neq -1$ .

Suppose firstly that  $L(x^2 + y^2) = 0$ . This happens just when  $x^2 + y^2 \equiv 0 \pmod{p}$ , and so  $y^2 \equiv -x^2 \pmod{p}$ . Suppose, in that case, that  $x \not\equiv 0 \pmod{p}$ . Then it follows that  $\frac{y^2}{x^2} \equiv -1 \pmod{p}$ . However,  $L(-1) = -1$ , so this is a contradiction, and thus  $x \equiv 0 \pmod{p}$ . It follows that  $y^2 \equiv 0 \pmod{p}$ , and thus  $y \equiv 0 \pmod{p}$ . As such,  $s = 0 + i0$ . Set  $r = 0 + i0$  also: then  $r^2 = s$ , trivially.

So now suppose  $L(x^2 + y^2) = 1$ . This means that at least one of  $x$  and  $y$  is non-zero modulo  $p$ , as otherwise we would have  $L(x^2 + y^2) = 0$ .

Thus far, so elementary - but now we reach the fiddly part. Let  $w = x + K(x^2 + y^2)$ . Can it be true that  $w \equiv 0 \pmod{p}$ ? The Reference Implementation assumes not, but this is not so.

$w \equiv 0 \pmod{p} \implies -x \equiv (\text{mod } p) \implies x^2 \equiv K(x^2 + y^2)^2 \equiv (x^2 + y^2)L(x^2 + y^2) \equiv x^2 + y^2 \pmod{p}$ . It follows that  $y \equiv 0 \pmod{p}$ , and thus  $-x \equiv K(x^2) \pmod{p}$  - and so  $L(x) = -1$ , as  $K(x^2) \equiv xL(x) \pmod{p}$  - thus,  $x$  is a quadratic non-residue in  $\mathbb{F}_p$ . This is exactly the case where  $s$  is a quadratic non-residue in  $\mathbb{F}_p$  (and hence we would expect its square root to be purely “imaginary”).

Now consider  $w' = x - K(x^2 + y^2)$ . When is  $w' \equiv 0 \pmod{p}$ ? An identical argument shows that it is when  $y \equiv 0 \pmod{p}$  and  $x$  is a quadratic residue in  $\mathbb{F}_p$  (non-zero by our assumption) - which corresponds to  $s$  being a quadratic residue in  $\mathbb{F}_p$  (and hence having a purely “real” root).

It follows, then, that we can never have  $w \equiv w' \equiv 0 \pmod{p}$ . That motivates the following definition: let

$$u \equiv \frac{x + tK(x^2 + y^2)}{2},$$

where  $t \in 1, -1$  is chosen such that  $u \not\equiv 0 \pmod{p}$ . Specifically, if  $w \not\equiv 0 \pmod{p}$ ,  $u = \frac{w}{2}$ , and otherwise  $u = \frac{w'}{2}$ .

Let  $\alpha = K(u)$ .  $\alpha^2 \equiv uL(u) \pmod{p}$ , and so it follows that  $\alpha \not\equiv 0 \pmod{p}$  either. Let  $\beta = \frac{y\alpha}{2u}$ . Then  $\beta \equiv \frac{y\alpha^2}{2u\alpha} \equiv \frac{yuL(u)}{2u\alpha} \equiv y\frac{L(u)}{2\alpha} \pmod{p}$ , and so it follows that  $2\alpha\beta \equiv yL(u) \pmod{p}$ .

Note that  $L(u)^2 = 1$ . It follows that we have  $2\alpha^2L(u) \equiv 2u \pmod{p}$ , and hence the following equivalence holds:

$$(2\alpha^2L(u) - x)^2 \equiv (2u - x)^2 \equiv t^2K(x^2 + y^2)^2 \equiv (x^2 + y^2)L(x^2 + y^2) \pmod{p}.$$

Thus, by the assumption, we have  $(2\alpha^2L(u) - x)^2 \equiv x^2 + y^2 \pmod{p}$ .

Expanding and cancelling the  $x^2$  from both sides, we get  $4\alpha^4 - 4\alpha^2L(u)x \equiv y^2 \pmod{p}$ .

Thus, rearranging, we get that  $xL(u) \equiv \alpha^2 - \frac{y^2}{4\alpha^2} \equiv \alpha - \frac{y}{2\alpha} \equiv \alpha^2 - \frac{yL(u)^2}{2\alpha} \equiv \alpha^2 - \beta^2$ .

Now,  $(\alpha + i\beta)^2 = \alpha^2 - \beta^2 + i2\alpha\beta = L(u)(x + iy) = L(u)s$ , where equality here is over  $\mathbb{F}_{p^2}$  and thus modulo  $p$ . Similarly,  $(\beta - i\alpha)^2 = \beta^2 - \alpha^2 - i2\alpha\beta = -L(u)s$ .

Thus, if  $\alpha^2 \equiv u \pmod{p}$ ,  $L(u) = 1$ , and thus if we set  $r = \alpha + i\beta$ ,  $r^2 = s$ . If  $\alpha^2 \not\equiv u \pmod{p}$ , then in fact  $\alpha^2 \equiv -u \pmod{p}$ ,  $L(u) = -1$ , and so it will follow that if we set  $r = \beta - i\alpha$ ,  $r^2 = s$ . This proves the result.  $\square$

**Remark.** We may slightly simplify the last part. If we set  $\beta' = \frac{y}{2\alpha}$ , then:

- In the  $L(u) = 1$  case,  $\beta' = \beta$  and thus  $r = \alpha + i\beta'$ .
- In the  $L(u) = -1$  case,  $\beta' = -\beta$ , and thus  $r = -\beta' - i\alpha$ . But then  $r' = \beta' + i\alpha$  is also a square root of  $s$ .

As such, if we set  $\alpha = K(u)$ ,  $\beta = \frac{y}{2\alpha}$ , then:

- If  $\alpha^2 \equiv u \pmod{p}$ ,  $\alpha + i\beta$  is a square root of  $s$ .
- Otherwise,  $\beta + i\alpha$  is a square root of  $s$ .

There is, as we have seen here, some slightly ambiguity about what “the” square root of  $s$  should be, and what the SIKE specification [] *does* do is define this.

**Definition 5.** Suppose  $s \in \mathbb{F}_{p^2}$  and there exists some  $r = \alpha + i\beta \in \mathbb{F}_{p^2}$  with  $r^2 = s$ , with  $\alpha$  and  $\beta$  considered as integers in  $[0, p-1]$ .

Then define

$$\sqrt{s} = \begin{cases} r & \alpha \neq 0, \alpha \equiv 0 \pmod{2}, \\ r & \alpha = 0, \beta \equiv 0 \pmod{2}, \\ -r & \text{otherwise.} \end{cases}$$

All of this suggests the following algorithm. In the following, all members of  $\mathbb{F}_p$  are considered as elements of  $[0, p-1]$ , with equality modulo  $p$ .

---

**Algorithm 1:** An algorithm for calculating square roots in  $\mathbb{F}_{p^2} = \frac{\mathbb{F}_p[i]}{i^2+1}$ , where  $p$  is a prime and  $p \equiv -1 \pmod{4}$ .

---

**Input:** An element  $s = x + iy$  of  $\mathbb{F}_{p^2}$ , with  $x, y \in \mathbb{F}_p$ , such that there exists some  $r \in \mathbb{F}_{p^2}$ ,  $r^2 = s$ . We may check if  $s$  is a valid input by checking that  $(x^2 + y^2)^{\frac{p-1}{2}} \not\equiv -1 \pmod{p}$ .

**Output:**  $\sqrt{s}$ , as defined above.

**if**  $x = 0$  **and**  $y = 0$  **then**

|  $\alpha \leftarrow 0$   
|  $\beta \leftarrow 0$

**else**

|  $t_0 \leftarrow (x^2 + y^2)^{\frac{p+1}{4}}$   
|  $u \leftarrow \frac{x+t_0}{2}$

**if**  $u = 0$  **then**

|  $u \leftarrow u - t_0$

$\alpha \leftarrow u^{\frac{p+1}{4}}$

$\beta \leftarrow \frac{y}{2\alpha}$

**if**  $\alpha^2 \neq u$  **then**

|  $t_1 \leftarrow \alpha$

|  $\alpha \leftarrow \beta$

|  $\beta \leftarrow t_1$

**if**  $\alpha \equiv 1 \pmod{2}$  **or**  $(\alpha = 0$  **and**  $\beta \equiv 1 \pmod{2})$  **then**

|  $\alpha \leftarrow -\alpha$

|  $\beta \leftarrow -\beta$

**return**  $\alpha + i\beta$

---

**Lemma 6.** *Algorithm 1 calculates  $\sqrt{s}$  as claimed.*

*Proof.* Follows from the theorem, the remark which follows it, and the definition of  $\sqrt{s}$ . □